# baseURI: https://linked.data.gov.au/def/csdm/commonpatterns
# imports: http://www.w3.org/2004/02/skos/core
# imports: http://www.w3.org/ns/dx/prof

@prefix : <https://linked.data.gov.au/def/csdm/commonpatterns/> .
@prefix dct: <http://purl.org/dc/terms/> .
@prefix ont: <https://linked.data.gov.au/def/csdm/commonpatterns> .
@prefix ontologyprojects: <http://teamwork.topbraidlive.org/ontologyprojects#> .
@prefix owl: <http://www.w3.org/2002/07/owl#> .
@prefix prof: <http://www.w3.org/ns/dx/prof/> .
@prefix rdf: <http://www.w3.org/1999/02/22-rdf-syntax-ns#> .
@prefix rdfs: <http://www.w3.org/2000/01/rdf-schema#> .
@prefix sh: <http://www.w3.org/ns/shacl#> .
@prefix skos: <http://www.w3.org/2004/02/skos/core#> .
@prefix teamwork: <http://topbraid.org/teamwork#> .
@prefix xsd: <http://www.w3.org/2001/XMLSchema#> .

ont:
  a owl:Ontology ;
  rdfs:label "Common implementation patterns not directly supported by other standards" ;
  # owl:imports <http://www.w3.org/2004/02/skos/core> ;
  # owl:imports <http://www.w3.org/ns/dx/prof> ;
.
:Common
  a owl:Class ;
  a sh:NodeShape ;
  rdfs:isDefinedBy ont: ;
  rdfs:label "Common Implementation Patterns" ;
  skos:definition "SuperClass for common implementations patterns not provided by existing standards" ;
  skos:prefLabel "Common Reusable Patterns" ;
.
:CompoundName
  a owl:Class ;
  a sh:NodeShape ;
  rdfs:isDefinedBy ont: ;
  rdfs:label "CompoundName" ;
  rdfs:subClassOf :Common ;
  rdfs:subClassOf [
      a owl:Restriction ;
      owl:minCardinality "1"^^xsd:nonNegativeInteger ;
      owl:onProperty dct:hasPart ;
    ] ;
  skos:definition "An ordered list of name parts. The order may be specified by either a list implementation, by implicit order defined in a formatting specification, or within a more explicit model of name part types." ;
  <http://xmlns.com/foaf/0.1/depiction> <https://surroundbitbucket.bitbucket.io/3d-cadastre/spec/CompoundName.png> ;
.
:Measure
  a owl:Class ;
  rdfs:isDefinedBy ont: ;
  rdfs:label "Qualified Measurement" ;
  rdfs:subClassOf :Common ;
  rdfs:subClassOf [
      a owl:Restriction ;
      owl:cardinality 1 ;
      owl:onProperty :value ;
    ] ;
  rdfs:subClassOf [
      a owl:Restriction ;
      owl:maxCardinality 1 ;
      owl:onProperty :qualityMeasure ;
    ] ;
.
:NamePart
  a owl:Class ;
  a sh:NodeShape ;
  rdfs:comment "Name Parts may be specialised by local business rules and support additional referential and syntactic requirements. Localised models may define implicit order for constructing a compound name if no format is specified in a containing CompoundName." ;
  rdfs:isDefinedBy ont: ;
  rdfs:label "Name Part" ;
  rdfs:subClassOf :Common ;
  rdfs:subClassOf [
      a owl:Restriction ;
      owl:cardinality "1"^^xsd:nonNegativeInteger ;
      owl:onProperty skos:prefLabel ;
    ] ;
  skos:definition "An ordered part of a compound name." ;
.
:RelevantJurisdictionalCodelist
  a owl:Class ;
  a sh:NodeShape ;
  rdfs:isDefinedBy ont: ;
  rdfs:label "Relevant Jurisdictional Codelist" ;
  rdfs:subClassOf skos:ConceptScheme ;
  rdfs:subClassOf :Common ;
  skos:definition "A codelist that will be defined in each implementing jurisdiction" ;
.
:Report
  a owl:Class ;
  a sh:NodeShape ;
  rdfs:isDefinedBy ont: ;
  rdfs:label "Report" ;
  rdfs:subClassOf prof:ResourceDescriptor ;
  rdfs:subClassOf :Common ;
  skos:definition "An arbitrary report of a known type, with metadata about its purpose and format as required." ;
  skos:editorialNote "Logical model using the ResourceDescriptor pattern from the Profiles vocabulary to allow specification of what form the report or document is in. " ;
.
:name
  a owl:ObjectProperty ;
  rdfs:isDefinedBy ont: ;
  rdfs:comment "a label property may be present on the subject with the preferred formatting of a compound name." ;
  rdfs:label "Name" ;
  rdfs:range :CompoundName ;
  skos:definition "A name composed of components according to localised implementation requirements." ;
.
:qualityMeasure
  a owl:DatatypeProperty ;
  rdfs:isDefinedBy ont: ;
  rdfs:label "Quality Measure" ;
  rdfs:range xsd:decimal ;
  skos:definition "a numeric quality measure" ;
  skos:scopeNote "This has not been fully modelled - a placeholder - for an ISO 19157 DQV concept" ;
.
:qualityClass
  a owl:ObjectProperty ;
  rdfs:isDefinedBy ont: ;
  rdfs:label "Quality Class" ;
  skos:scopeNote "A reference to a code indicating a quality class" ;
.
:value
  a owl:DatatypeProperty ;
  rdfs:isDefinedBy ont: ;
  rdfs:label "value" ;
  rdfs:range xsd:decimal ;
.
