# baseURI: https://linked.data.gov.au/def/csdm/container
# imports: https://linked.data.gov.au/def/csdm/geometry
# imports: https://linked.data.gov.au/def/csdm/parcels
# imports: https://linked.data.gov.au/def/csdm/surveyfeatures
# imports: https://linked.data.gov.au/def/csdm/surveyobs
# imports: https://linked.data.gov.au/def/csdm/surveyprov
# imports: https://www.opengis.net/def/profiles/geosparql3d
# prefix: ont

@prefix com:       <https://linked.data.gov.au/def/csdm/commonpatterns/> .
@prefix container: <https://linked.data.gov.au/def/csdm/container/> .
@prefix dct:       <http://purl.org/dc/terms/> .
@prefix geometry:  <https://linked.data.gov.au/def/csdm/geometry/> .
@prefix ont:       <https://linked.data.gov.au/def/csdm/container> .
@prefix owl:       <http://www.w3.org/2002/07/owl#> .
@prefix parcel:    <https://linked.data.gov.au/def/csdm/parcels/> .
@prefix rdf:       <http://www.w3.org/1999/02/22-rdf-syntax-ns#> .
@prefix rdfs:      <http://www.w3.org/2000/01/rdf-schema#> .
@prefix schema:    <https://schema.org/> .
@prefix sh:        <http://www.w3.org/ns/shacl#> .
@prefix skos:      <http://www.w3.org/2004/02/skos/core#> .
@prefix surv:      <https://linked.data.gov.au/def/csdm/surveyfeatures/> .
@prefix surveyobs: <https://linked.data.gov.au/def/csdm/surveyobs/> .
@prefix survprov:  <https://linked.data.gov.au/def/csdm/surveyprov/> .
@prefix xsd:       <http://www.w3.org/2001/XMLSchema#> .

ont:
    a               owl:Ontology ;
    rdfs:label      "Survey Plan Container Model" ;
    # owl:imports <https://linked.data.gov.au/def/csdm/geometry> ;
    # owl:imports <https://linked.data.gov.au/def/csdm/parcels> ;
    # owl:imports <https://linked.data.gov.au/def/csdm/surveyfeatures> ;
    # owl:imports <https://linked.data.gov.au/def/csdm/surveyobs> ;
    # owl:imports <https://linked.data.gov.au/def/csdm/surveyprov> ;
    # owl:imports <https://www.opengis.net/def/profiles/geosparql3d> ;
    skos:definition "Import closure for 3D model packages and aggregation containers for exchange objects." ;
    schema:image    [ a              schema:ImageObject ;
                      sh:order       0 ;
                      schema:caption "Diagram of the class Container." ;
                      schema:contentUrl
                                     "https://surroundbitbucket.bitbucket.io/3d-cadastre/spec/Container.png"^^xsd:anyURI ; ] ;
.

container:CSD
    a                  owl:Class ;
    a                  sh:NodeShape ;
    rdfs:isDefinedBy   ont: ;
    rdfs:label         "Cadastral Survey Dataset" ;
    rdfs:subClassOf    container:ClassIn3DCadastre ;
    rdfs:subClassOf    survprov:SurveyEntity ;
    skos:definition    "The set of cadastral survey data necessary to integrate a cadastral survey into, or transfer survey observations from, a cadastral database. A CSD identifier may be used to reference a previous survey." ;
    skos:definition    "This exists without adequate definition in both LandInfra and landXML" ;
    schema:workExample [ a                     schema:TextObject ;
                         schema:encodingFormat "text/turtle" ;
                         schema:text           """
      examples1:SurveyExample
        a container:CSD ;
        rdfs:label "Example Cadastral Survey Dataset" ;
        prov:wasGeneratedBy surveyobs_examples:surveyActivity1 ;
        container:calculatedObservations surveyobs_examples:calculated_observations ;
        container:occupationFeatures surveyobs_examples:fence1 ;
        container:referencedCSD surveyobs_examples:csd2 ;
        container:vectorObservations surveyobs_examples:vector_observations ;
      .
    """ ; ] ;
    skos:scopeNote     "Cadastral Survey Datasets may reference data from previous surveys, the extracted subset for each relevant previous survey is contained within a separate CSD object referenced by the CSD being submitted. Implementations will determine how these make be packaged, conceptually referenced CSDs are seen as a property of any given CSD" ;
    schema:image       [ a              schema:ImageObject ;
                         sh:order       0 ;
                         schema:caption "Diagram for Cadastral Survey Dataset." ;
                         schema:contentUrl
                                        "https://icsm-au.github.io/3d-csdm-design/2022/spec_files/CSD_logical.png"^^xsd:anyURI ; ] ;
.

container:ClassIn3DCadastre
    a               owl:Class ;
    rdfs:label      "Class defined in 3D Cadastre Model" ;
    rdfs:subClassOf container:ModelledElement ;
.

container:GeoSPARQL-3D
    a               owl:Class ;
    a               sh:NodeShape ;
    rdfs:label      "GeoSPARQL 1.2 (3D profile)" ;
    rdfs:subClassOf container:ClassIn3DCadastre ;
    skos:definition "This class represents a container for objects described by the 3D profile of ISO19107 as a GeoSPARQL 1.2 extension candidate." ;
.

container:ModelledElement
    a               owl:Class ;
    a               sh:NodeShape ;
    rdfs:label      "SelectableModelElement" ;
    rdfs:subClassOf owl:Thing ;
.

container:StandardClass
    a               owl:Class ;
    rdfs:label      "Key Class used by 3D Cadastre Model" ;
    rdfs:subClassOf container:ModelledElement ;
    skos:definition "This class is just to provide a highlight for key class types used by 3D Cadastre model" ;
.

container:bearingRotation
    a          rdf:Property ;
    rdfs:label "bearingRotation" ;
    skos:definition
               "The bearing rotation to apply to all vectors in a CSD relative to a referential context such as a CSD adopting bearings from this CSD." ;
.

container:horizontalCRS
    a               rdf:Property ;
    rdfs:label      "horizontal CRS" ;
    skos:definition "The CRS  to assume for all horizontal coordinates in scope of this object." ;
.

container:compoundCRS
    a               rdf:Property ;
    rdfs:label      "Compound CRS" ;
    skos:definition "The CRS to assume for both horizontal and vertical coordinates in scope of this object." ;
.

container:adminUnit
    a               rdf:Property ;
    rdfs:label      "Administration Unit" ;
    skos:definition "Qualified reference to Administration Unit identifiers." ;
.

container:occupationFeatures
    a               owl:ObjectProperty ;
    dct:description "Occupation Features referenced in occupation observations or by specific Observation Marks" ;
    rdfs:label      "Occupation Features" ;
    rdfs:range      geometry:FeatureCollection ;
.

container:occupationObservations
    a          owl:ObjectProperty ;
    a          sh:PropertyShape ;
    dct:description
               "the set of observations about the nature of occupation present for survey features. Note that the relative positions of occupation features may be present as vector observations." ;
    rdfs:label "Observations on Occupation Features" ;
    rdfs:range <http://www.w3.org/ns/sosa/ObservationCollection> ;
.

container:parcels
    a          owl:ObjectProperty ;
    rdfs:label "Parcels" ;
    dct:description
               "the set of Parcels defined or re-surveyed by this survey. These reference vectors which in turn reference the points coordinate geometry of the survey, using topological relationships to these points via the \"id\" property." ;
    rdfs:range geometry:FeatureCollection ;
.

container:points
    a          owl:ObjectProperty ;
    rdfs:label "Survey Points" ;
    dct:description
               "the set of survey points defined or re-surveyed by this survey. These contain all the coordinate geometry of the survey, other features are defined using topological relationships to these points by the \"id\" property." ;
    rdfs:range geometry:FeatureCollection ;
.

container:referencedCSD
    a               rdf:Property ;
    dct:description "Is a CSD container that references existing CSD survey features and observations surveyed and /or used/adopted as part of the survey definition for the CSD. In short, it is a list of previous surveys (CSD) used in the current survey. Note that the implementation may be a set of empty (shell) CSDs containing minimal metadata and a CSD referencing this will contain the relevant set of adopted observations and points" ;
    rdfs:label      "Referenced CSD" ;
    skos:definition "A CSD containing referenced survey features and observations" ;
.

container:surveyProvenance
    a               owl:ObjectProperty ;
    dct:description "The set of activities, actors and related information objects describing the provenance of an object " ;
    rdfs:label      "Provenance" ;
    rdfs:range      <http://www.w3.org/ns/prov#Bundle> ;
.

container:vectorObservations
    a          owl:ObjectProperty ;
    a          sh:PropertyShape ;
    dct:description
               "the set of observed vectors defined or re-surveyed by this survey - adopted vectors will be present in the context of the original CSD they are adopted from to preserve metadata." ;
    rdfs:label "Vector Observations" ;
    rdfs:range <http://www.w3.org/ns/sosa/ObservationCollection> ;
.

container:verticalDatum
    a               rdf:Property ;
    rdfs:label      "verticalDatum" ;
    skos:definition "The verticalDatum to assume for all height values in scope of this object." ;
.

geometry:3DSpatialUnit
    rdfs:subClassOf container:GeoSPARQL-3D ;
.

geometry:BoundaryFeature
    rdfs:subClassOf container:GeoSPARQL-3D ;
.

geometry:SolidGeometry
    rdfs:subClassOf container:GeoSPARQL-3D ;
.

parcel:ParcelModel
    rdfs:subClassOf container:ClassIn3DCadastre ;
.

surv:CadastralFeature
    rdfs:subClassOf container:ClassIn3DCadastre ;
.

surv:SurveyPurpose
    a                owl:Class ;
    rdfs:label       "Survey Purpose Code" ;
    rdfs:subClassOf  com:RelevantJurisdictionalCodelist ;
    skos:definition  "A controlled vocabulary term for the purpose of a survey" ;
.

container:purpose
    a               owl:ObjectProperty ;
    rdfs:label      "Survey Purpose" ;
    skos:definition "the purpose of a survey" ;
    rdfs:range      skos:Concept ;
.

surveyobs:Measure
    a               owl:Class ;
    a               sh:NodeShape ;
    rdfs:label      "GeoSPARQL 1.2 (3D profile)" ;
    rdfs:subClassOf container:StandardClass ;
.

surveyobs:SurveyObservation
    rdfs:subClassOf <http://www.w3.org/ns/sosa/Observation> ;
    rdfs:subClassOf container:ClassIn3DCadastre ;
.

survprov:SurveyProvenanceObject
    rdfs:subClassOf container:ClassIn3DCadastre ;
.
