# baseURI: https://linked.data.gov.au/def/csdm/surveyfeatures
# imports: https://linked.data.gov.au/def/csdm/commonpatterns
# imports: https://linked.data.gov.au/def/csdm/geometry

@prefix : <https://linked.data.gov.au/def/csdm/surveyfeatures/> .
@prefix com: <https://linked.data.gov.au/def/csdm/commonpatterns/> .
@prefix dct: <http://purl.org/dc/terms/> .
@prefix foaf: <http://xmlns.com/foaf/0.1/> .
@prefix geometry: <https://linked.data.gov.au/def/csdm/geometry/> .
@prefix landinfra: <http://www.opengis.net/def/schema/landinfra/core/> .
@prefix ont: <https://linked.data.gov.au/def/csdm/surveyfeatures> .
@prefix owl: <http://www.w3.org/2002/07/owl#> .
@prefix prof: <http://www.w3.org/ns/dx/prof/> .
@prefix rdf: <http://www.w3.org/1999/02/22-rdf-syntax-ns#> .
@prefix rdfs: <http://www.w3.org/2000/01/rdf-schema#> .
@prefix schema: <https://schema.org/> .
@prefix sh: <http://www.w3.org/ns/shacl#> .
@prefix skos: <http://www.w3.org/2004/02/skos/core#> .
@prefix specs: <https://linked.data.gov.au/def/csdm/impspecs/> .
@prefix xsd: <http://www.w3.org/2001/XMLSchema#> .

ont:
  a owl:Ontology ;
  skos:prefLabel "Survey Features Model"@en ;
  # owl:imports <https://linked.data.gov.au/def/csdm/commonpatterns> ;
  # owl:imports <https://linked.data.gov.au/def/csdm/geometryprim> ;
  skos:definition "Feature Types defined by Cadastral Surveys"@en ;
  <https://data.surroundaustralia.com/def/class-example-shapes/implExample> [
      a prof:ResourceDescriptor ;
      dct:conformsTo specs:ClassContextDiagram ;
      dct:conformsTo specs:UML ;
      rdfs:label "Package Dependencies Diagram" ;
      prof:hasArtifact "https://surroundbitbucket.bitbucket.io/3d-cadastre/spec/survey_package_diagram.png" ;
    ] ;
.
:AdoptedVector
  a owl:Class ;
  rdfs:isDefinedBy ont: ;
  skos:prefLabel "Adopted Vector"@en ;
  rdfs:subClassOf :SurveyedLine ;
  skos:definition "A vector included in a CSD that has previously been observed and included in an existing CSD or Survey Plan."@en ;
.
:AllowableCoordinateReferenceSystem
  a owl:Class ;
  rdfs:isDefinedBy ont: ;
  skos:prefLabel "Allowable Coordinate Reference System"@en ;
  rdfs:subClassOf com:RelevantJurisdictionalCodelist ;
  skos:definition "The set of CRS supported by a cadastral system for survey lodgement."^^rdf:HTML ;
.
:Angle
  a owl:Class ;
  rdfs:isDefinedBy ont: ;
  skos:prefLabel "Angle Measurement"@en ;
  rdfs:subClassOf com:Measure ;
.
:BoundaryMark
  a owl:Class ;
  rdfs:isDefinedBy ont: ;
  skos:prefLabel "Boundary Mark"@en ;
  rdfs:subClassOf :SurveyMark ;
  skos:definition """Means a location that defines a boundary corner or boundary alignment. The location will be physically marked unless the location is obstructed by a structure that can not be marked.

A boundary mark MAY be a Geodetic Reference Mark.""" ;
.
:CadastralFeature
  a owl:Class ;
  rdfs:isDefinedBy ont: ;
  skos:prefLabel "Cadastral Feature"@en ;
  rdfs:subClassOf <http://www.opengis.net/ont/geosparql#Feature> ;
  skos:definition "This is an abstract feature to identify elements of the Cadastral Survey Conceptual Model"@en ;
  foaf:depiction <https://surroundbitbucket.bitbucket.io/3d-cadastre/spec/SurveyFeatures.png> ;
  schema:image [
      a schema:ImageObject ;
      sh:order 0 ;
      schema:caption "Diagram for Cadastral Feature." ;
      schema:contentUrl "https://icsm-au.github.io/3d-csdm-design/2022/spec_files/SurveyFeatures.png"^^xsd:anyURI ;
  ] ;
.
:CadastralMark
  a owl:Class ;
  rdfs:isDefinedBy ont: ;
  skos:prefLabel "Cadastral Mark"@en ;
  rdfs:subClassOf :SurveyMark ;
  skos:definition """Any survey mark placed or observed as part of a cadastral survey that is not a boundary mark or a geodetic reference mark
""" ;
.
:Distance
  a owl:Class ;
  rdfs:isDefinedBy ont: ;
  skos:prefLabel "Distance Measurement"@en ;
  rdfs:subClassOf com:Measure ;
.
:GeodeticReferenceMark
  a owl:Class ;
  rdfs:isDefinedBy ont: ;
  skos:prefLabel "Geodetic Reference Mark"@en ;
  rdfs:subClassOf :SurveyMark ;
  skos:definition "Means a mark that connects a survey to the jurisdictional geodetic network, vertical or horizontal."@en ;
.
:Monument
  a owl:Class ;
  rdfs:isDefinedBy ont: ;
  skos:prefLabel "Monument"@en ;
  rdfs:subClassOf :CadastralFeature ;
  rdfs:subClassOf [
      a owl:Restriction ;
      owl:cardinality "1"^^xsd:nonNegativeInteger ;
      owl:onProperty :condition ;
    ] ;
  skos:definition "An object that is placed in the ground, or referred to, for the purpose of identifying a survey point in a cadastral survey."^^rdf:HTML ;
.
:MonumentCondition
  a owl:Class ;
  rdfs:isDefinedBy ont: ;
  skos:prefLabel "Monument Condition"@en ;
  rdfs:subClassOf com:RelevantJurisdictionalCodelist ;
  skos:definition "Means the state of a survey mark at the time it is found during a cadastral survey."@en ;
.
:MonumentForm
  a owl:Class ;
  rdfs:isDefinedBy ont: ;
  skos:prefLabel "Monument Form"@en ;
  rdfs:subClassOf com:RelevantJurisdictionalCodelist ;
  skos:definition "Physical Form of a monument"@en ;
.
:NoOccupation
  a owl:Class ;
  rdfs:isDefinedBy ont: ;
  skos:prefLabel "No Occupation"@en ;
  rdfs:subClassOf :Occupation ;
  skos:definition "Special case where no occupation is observable."@en ;
.
:ObservedVector
  a owl:Class ;
  rdfs:isDefinedBy ont: ;
  skos:prefLabel "Observed Vector"@en ;
  rdfs:subClassOf :SurveyedLine ;
  skos:definition "A vector consisting of one or more reduced and/or adjusted observed measurements.  Observations may include calculation procedures."@en ;
  schema:image [
      a schema:ImageObject ;
      sh:order 0 ;
      schema:caption "Diagram for Observed Vector." ;
      schema:contentUrl "https://icsm-au.github.io/3d-csdm-design/2022/spec_files/ObservedVector.png"^^xsd:anyURI ;
  ] ;
.
:Occupation
  a owl:Class ;
  rdfs:isDefinedBy ont: ;
  skos:prefLabel "Occupation Feature"@en ;
  rdfs:subClassOf <http://www.opengis.net/ont/geosparql#Feature> ;
  skos:definition """Means those long-established features that might be used to determine the limits of an occupierâ€™s land, and that are used to exclude possession by others, e.g., fences, walls, trees, hedges, buildings, ditches, or other artificial things; and natural land features such as a water body.

An occupation feature is disjoint from (has no common elements with) a boundary.""" ;
.
:OccupationMark
  a owl:Class ;
  rdfs:isDefinedBy ont: ;
  skos:prefLabel "Occupation Mark"@en ;
  rdfs:subClassOf :SurveyPoint ;
  skos:definition "Means a mark used for a cadastral survey to define the location of an occupation feature near a cadastral boundary"@en ;
  skos:editorialNote "Occupation Marks are not monumented but may be described. Observed Vectors or Direct Position Observations determine the location of the mark." ;
.
:SurveyMark
  a owl:Class ;
  rdfs:isDefinedBy ont: ;
  skos:prefLabel "Survey Mark"@en ;
  rdfs:subClassOf :SurveyPoint ;
  rdfs:subClassOf [
      a owl:Restriction ;
      owl:minCardinality "1"^^xsd:nonNegativeInteger ;
      owl:onProperty com:name ;
    ] ;
  rdfs:subClassOf [
      a owl:Restriction ;
      owl:minCardinality "1"^^xsd:nonNegativeInteger ;
      owl:onProperty :monumentedBy ;
    ] ;
  owl:equivalentClass landinfra:SurveyMark ;
  skos:definition "A SurveyMark is a physically located object which by its form defines a point on the surface of the Earth and which is stable during surveying operations"@en ;
  skos:editorialNote "The purpose of the mark is relative the CSD - so the same identified object may have different types in different CSDs - in which case how does the aggregated data record the purpose?" ;
  foaf:depiction <https://surroundbitbucket.bitbucket.io/3d-cadastre/spec/surveymark.png> ;
.
:SurveyPoint
  a owl:Class ;
  rdfs:isDefinedBy ont: ;
  skos:prefLabel "Survey Point"@en ;
  rdfs:subClassOf :CadastralFeature ;
  skos:definition "Any point of interest in a survey. It may relate to a boundary corner (marked or unmarked), a cadastral mark, a geodetic reference mark, or an occupation mark"@en ;
.
:SurveyPointProvenance
  a owl:Class ;
  rdfs:isDefinedBy ont: ;
  skos:prefLabel "Survey Point Provenance"@en ;
  rdfs:subClassOf com:RelevantJurisdictionalCodelist ;
  skos:definition "A survey point MAY state the source of the point, and that it may be declared using a relevant jurisdictional code list or a jurisdictional pattern"@en ;
.
:SurveyPointPurpose
  a owl:Class ;
  rdfs:isDefinedBy ont: ;
  skos:prefLabel "Survey Point Purpose"@en ;
  rdfs:subClassOf com:RelevantJurisdictionalCodelist ;
  skos:definition "The purpose of a recorded survey point in relation to the current survey activity"@en ;
.
:SurveyPointQuality
  a owl:Class ;
  rdfs:isDefinedBy ont: ;
  skos:prefLabel "Survey Point Quality"@en ;
  rdfs:subClassOf com:RelevantJurisdictionalCodelist ;
  skos:definition "The quality/accuracy class of a recorded survey point in accordance with the relevant jurisdiction standard"@en ;
.
:SurveyPointState
  a owl:Class ;
  rdfs:isDefinedBy ont: ;
  skos:prefLabel "Survey Point State"@en ;
  rdfs:subClassOf com:RelevantJurisdictionalCodelist ;
  skos:definition "The state of a recorded survey point in accordance with the relevant jurisdiction standard"@en ;
  skos:editorialNote "The distinction between survey point state and monument condition may require further explanations and examples." ;
.
:SurveyedLine
  a owl:Class ;
  rdfs:isDefinedBy ont: ;
  skos:prefLabel "Surveyed Line"@en ;
  rdfs:subClassOf :CadastralFeature ;
  skos:definition "A line of survey between an instrument location and a target point"@en ;
  skos:definition "Means a geometric object that has magnitude (or length) and direction. For a cadastral survey system the geometric object consists of a set of reduced survey observations between two survey points. "^^rdf:HTML ;
  skos:scopeNote "To keep consistent with the paradigm of a line existing between two points, and to avoid duplication of information the instrument location is a special type of feature with a point geometry that may have several related observations and a link to setup information. " ;
.
:Terrain
  a owl:Class ;
  rdfs:isDefinedBy ont: ;
  skos:prefLabel "Terrain"@en ;
  rdfs:subClassOf :Occupation ;
.
:VectorDeterminationMethod
  a owl:Class ;
  rdfs:isDefinedBy ont: ;
  skos:prefLabel "Vector Determination Method"@en ;
  rdfs:subClassOf com:RelevantJurisdictionalCodelist ;
  skos:definition "Each vector MAY state how it was defined using the relevant jurisdictional code list"@en ;
.
:condition
  a rdf:Property ;
  skos:prefLabel "monument condition"@en ;
  rdfs:range :MonumentCondition ;
.
:distance
  a owl:ObjectProperty ;
  rdfs:domain :SurveyedLine ;
  skos:prefLabel "Distance"@en ;
  rdfs:range :Distance ;
  skos:altLabel "Slope Distance" ;
  skos:definition "The line of sight distance between the instrument and target point"@en ;
.
:form
  a rdf:Property ;
  skos:prefLabel "Monument physical form"@en ;
  rdfs:range :MonumentForm ;
  skos:definition "Physical form of monument using code list"@en ;
.
:from
  a owl:ObjectProperty ;
  skos:prefLabel "from"@en ;
  rdfs:range :SurveyPoint ;
  skos:definition "Start point for a survey line"@en ;
.
:horizontalAngle
  a owl:ObjectProperty ;
  rdfs:domain :SurveyedLine ;
  skos:prefLabel "horizontal angle"@en ;
  rdfs:range :Angle ;
  skos:definition "The horizontal angle of the target point relative to the setup bearing"@en ;
.
:monumentedBy
  a owl:ObjectProperty ;
  skos:prefLabel "monumented by"@en ;
  skos:definition "Reference to physical monument description"@en ;
.
:provenance
  a rdf:Property ;
  skos:prefLabel "provenance"@en ;
  rdfs:range :SurveyPointProvenance ;
  skos:definition "Survey point provenance"@en ;
.
:purpose
  a owl:ObjectProperty ;
  skos:prefLabel "purpose"@en ;
  skos:definition "Purpose of an entity using relevant codelist"@en ;
.

:vectorPurpose
  a owl:ObjectProperty ;
  skos:prefLabel "purpose for a survey vector"@en ;
  skos:definition "Purpose of vector, using relevant codelist"@en ;
.

:references
  a owl:objectProperty ;
  skos:prefLabel "references"@en ;
.
:replaces
  a owl:ObjectProperty ;
  rdfs:domain :Monument ;
  skos:prefLabel "replaces"@en ;
  rdfs:range :Monument ;
  skos:definition "Reference to description of previous monument"@en ;
.
:setup
  a owl:DatatypeProperty ;
  skos:prefLabel "setup"@en ;
.
:state
  a owl:ObjectProperty ;
  rdfs:domain :SurveyMark ;
  skos:prefLabel "state"@en ;
  rdfs:range :SurveyPointState ;
  skos:definition "State of survey point"@en ;
.
:target
  a owl:ObjectProperty ;
  skos:prefLabel "target"@en ;
  rdfs:range :SurveyPoint ;
  skos:definition "Target (end) point for a survey line"@en ;
.
:verticalAngle
  a owl:ObjectProperty ;
  rdfs:domain :SurveyedLine ;
  skos:prefLabel "vertical angle"@en ;
  rdfs:range :Angle ;
  skos:definition "The horizontal angle of the target point relative to the setup bearing"@en ;
.
